code/hash/Hacl.Hash.MD.fsti
@@ -3,6 +3,14 @@ module Hacl.Hash.MD
 open Hacl.Hash.Definitions
 open Spec.Hash.Definitions
 
+module U32 = FStar.UInt32
+
+noextract inline_for_extraction
+val len_add32 (a: hash_alg{is_md a})
+  (prev_len: len_t a)
+  (input_len: U32.t { (U32.v input_len + len_v a prev_len) `less_than_max_input_length` a }):
+  x:len_t a { len_v a x = len_v a prev_len + U32.v input_len }
+
 noextract inline_for_extraction
 val mk_update_multi: a:hash_alg{is_md a} -> update:update_st (|a, ()|) -> update_multi_st (|a, ()|)
 
