specs/lemmas/Spec.Hash.Incremental.fsti
@@ -141,5 +141,7 @@ val blake2_is_hash_incremental
     S.equal (Blake2.blake2 (to_blake_alg a) input kk k (Spec.Blake2.max_output (to_blake_alg a)))
             (hash_incremental a input))
 
+val sha3_state_is_hash_state: squash (words_state' SHA3_256 == Spec.SHA3.state)
+
 val hash_is_hash_incremental (a: hash_alg) (input: bytes { S.length input `less_than_max_input_length` a }):
   Lemma (S.equal (hash a input) (hash_incremental a input))
